modernized syntax translations, using mostly abbreviation/notation; minor tuning;

src/HOL/Bali/Name.thy
@@ -20,13 +20,11 @@ datatype ename        --{* expression name *}
 datatype lname        --{* names for local variables and the This pointer *}
         = EName ename 
         | This
-syntax   
-  VName  :: "vname \<Rightarrow> lname"
-  Result :: lname
+abbreviation VName   :: "vname \<Rightarrow> lname"
+      where "VName n == EName (VNam n)"
 
-translations
-  "VName n" == "EName (VNam n)"
-  "Result"  == "EName Res"
+abbreviation Result :: lname
+      where "Result == EName Res"
 
 datatype xname          --{* names of standard exceptions *}
         = Throwable
