src/HOL/Bali/AxSem.thy
@@ -6,7 +6,6 @@
 header {* Axiomatic semantics of Java expressions and statements 
           (see also Eval.thy)
         *}
-
 theory AxSem imports Evaln TypeSafe begin
 
 text {*
@@ -39,14 +38,15 @@ restrictions:
 *}
 
 types  res = vals --{* result entry *}
-syntax
-  Val  :: "val      \<Rightarrow> res"
-  Var  :: "var      \<Rightarrow> res"
-  Vals :: "val list \<Rightarrow> res"
-translations
-  "Val  x"     => "(In1 x)"
-  "Var  x"     => "(In2 x)"
-  "Vals x"     => "(In3 x)"
+
+abbreviation (input)
+  Val where "Val x == In1 x"
+
+abbreviation (input)
+  Var where "Var x == In2 x"
+
+abbreviation (input)
+  Vals where "Vals x == In3 x"
 
 syntax
   "_Val"    :: "[pttrn] => pttrn"     ("Val:_"  [951] 950)
@@ -54,9 +54,9 @@ syntax
   "_Vals"   :: "[pttrn] => pttrn"     ("Vals:_" [951] 950)
 
 translations
-  "\<lambda>Val:v . b"  == "(\<lambda>v. b) \<circ> the_In1"
-  "\<lambda>Var:v . b"  == "(\<lambda>v. b) \<circ> the_In2"
-  "\<lambda>Vals:v. b"  == "(\<lambda>v. b) \<circ> the_In3"
+  "\<lambda>Val:v . b"  == "(\<lambda>v. b) \<circ> CONST the_In1"
+  "\<lambda>Var:v . b"  == "(\<lambda>v. b) \<circ> CONST the_In2"
+  "\<lambda>Vals:v. b"  == "(\<lambda>v. b) \<circ> CONST the_In3"
 
   --{* relation on result values, state and auxiliary variables *}
 types 'a assn   =        "res \<Rightarrow> state \<Rightarrow> 'a \<Rightarrow> bool"
@@ -105,10 +105,9 @@ apply (rule ext)
 apply auto
 done
 
-syntax
-  Normal     :: "'a assn \<Rightarrow> 'a assn"
-translations
-  "Normal P" == "P \<and>. normal"
+abbreviation
+  Normal :: "'a assn \<Rightarrow> 'a assn"
+  where "Normal P == P \<and>. normal"
 
 lemma peek_and_Normal [simp]: "peek_and (Normal P) p = Normal (peek_and P p)"
 apply (rule ext)
@@ -207,9 +206,9 @@ constdefs
  "peek_res Pf \<equiv> \<lambda>Y. Pf Y Y"
 
 syntax
-"@peek_res"  :: "pttrn \<Rightarrow> 'a assn \<Rightarrow> 'a assn"            ("\<lambda>_:. _" [0,3] 3)
+  "_peek_res" :: "pttrn \<Rightarrow> 'a assn \<Rightarrow> 'a assn"            ("\<lambda>_:. _" [0,3] 3)
 translations
-  "\<lambda>w:. P"   == "peek_res (\<lambda>w. P)"
+  "\<lambda>w:. P"   == "CONST peek_res (\<lambda>w. P)"
 
 lemma peek_res_def2 [simp]: "peek_res P Y = P Y Y"
 apply (unfold peek_res_def)
@@ -268,9 +267,9 @@ constdefs
  "peek_st P \<equiv> \<lambda>Y s. P (store s) Y s"
 
 syntax
-"@peek_st"   :: "pttrn \<Rightarrow> 'a assn \<Rightarrow> 'a assn"            ("\<lambda>_.. _" [0,3] 3)
+  "_peek_st"   :: "pttrn \<Rightarrow> 'a assn \<Rightarrow> 'a assn"            ("\<lambda>_.. _" [0,3] 3)
 translations
-  "\<lambda>s.. P"   == "peek_st (\<lambda>s. P)"
+  "\<lambda>s.. P"   == "CONST peek_st (\<lambda>s. P)"
 
 lemma peek_st_def2 [simp]: "(\<lambda>s.. Pf s) Y s = Pf (store s) Y s"
 apply (unfold peek_st_def)
@@ -386,33 +385,31 @@ something like triple = \<forall>'a. triple ('a assn) term ('a assn)   **)
                                         ("{(1_)}/ _>/ {(1_)}"      [3,65,3]75)
 types    'a triples = "'a triple set"
 
-syntax
-
+abbreviation
   var_triple   :: "['a assn, var         ,'a assn] \<Rightarrow> 'a triple"
                                          ("{(1_)}/ _=>/ {(1_)}"    [3,80,3] 75)
+  where "{P} e=> {Q} == {P} In2  e> {Q}"
+
+abbreviation
   expr_triple  :: "['a assn, expr        ,'a assn] \<Rightarrow> 'a triple"
                                          ("{(1_)}/ _->/ {(1_)}"    [3,80,3] 75)
+  where "{P} e-> {Q} == {P} In1l e> {Q}"
+
+abbreviation
   exprs_triple :: "['a assn, expr list   ,'a assn] \<Rightarrow> 'a triple"
                                          ("{(1_)}/ _#>/ {(1_)}"    [3,65,3] 75)
+  where "{P} e#> {Q} == {P} In3  e> {Q}"
+
+abbreviation
   stmt_triple  :: "['a assn, stmt,        'a assn] \<Rightarrow> 'a triple"
                                          ("{(1_)}/ ._./ {(1_)}"     [3,65,3] 75)
+  where "{P} .c. {Q} == {P} In1r c> {Q}"
 
-syntax (xsymbols)
-
-  triple       :: "['a assn, term        ,'a assn] \<Rightarrow> 'a triple"
-                                         ("{(1_)}/ _\<succ>/ {(1_)}"     [3,65,3] 75)
-  var_triple   :: "['a assn, var         ,'a assn] \<Rightarrow> 'a triple"
-                                         ("{(1_)}/ _=\<succ>/ {(1_)}"    [3,80,3] 75)
-  expr_triple  :: "['a assn, expr        ,'a assn] \<Rightarrow> 'a triple"
-                                         ("{(1_)}/ _-\<succ>/ {(1_)}"    [3,80,3] 75)
-  exprs_triple :: "['a assn, expr list   ,'a assn] \<Rightarrow> 'a triple"
-                                         ("{(1_)}/ _\<doteq>\<succ>/ {(1_)}"    [3,65,3] 75)
-
-translations
-  "{P} e-\<succ> {Q}" == "{P} In1l e\<succ> {Q}"
-  "{P} e=\<succ> {Q}" == "{P} In2  e\<succ> {Q}"
-  "{P} e\<doteq>\<succ> {Q}" == "{P} In3  e\<succ> {Q}"
-  "{P} .c. {Q}" == "{P} In1r c\<succ> {Q}"
+notation (xsymbols)
+  triple  ("{(1_)}/ _\<succ>/ {(1_)}"     [3,65,3] 75) and
+  var_triple  ("{(1_)}/ _=\<succ>/ {(1_)}"    [3,80,3] 75) and
+  expr_triple  ("{(1_)}/ _-\<succ>/ {(1_)}"    [3,80,3] 75) and
+  exprs_triple  ("{(1_)}/ _\<doteq>\<succ>/ {(1_)}"    [3,65,3] 75)
 
 lemma inj_triple: "inj (\<lambda>(P,t,Q). {P} t\<succ> {Q})"
 apply (rule inj_onI)
@@ -436,26 +433,25 @@ consts
     ax_valids :: "prog \<Rightarrow> 'b triples \<Rightarrow> 'a triples \<Rightarrow> bool"
                                                 ("_,_|\<Turnstile>_"   [61,58,58] 57)
 
-syntax
-
+abbreviation
  triples_valid:: "prog \<Rightarrow> nat \<Rightarrow>         'a triples \<Rightarrow> bool"
                                                 (  "_||=_:_" [61,0, 58] 57)
-     ax_valid :: "prog \<Rightarrow>  'b triples \<Rightarrow> 'a triple  \<Rightarrow> bool"
+ where "G||=n:ts == Ball ts (triple_valid G n)"
+
+abbreviation
+ ax_valid :: "prog \<Rightarrow>  'b triples \<Rightarrow> 'a triple  \<Rightarrow> bool"
                                                 ( "_,_|=_"   [61,58,58] 57)
+ where "G,A |=t == G,A|\<Turnstile>{t}"
 
-syntax (xsymbols)
-
- triples_valid:: "prog \<Rightarrow> nat \<Rightarrow>         'a triples \<Rightarrow> bool"
-                                                (  "_|\<Turnstile>_:_" [61,0, 58] 57)
-     ax_valid :: "prog \<Rightarrow>  'b triples \<Rightarrow> 'a triple  \<Rightarrow> bool"
-                                                ( "_,_\<Turnstile>_"   [61,58,58] 57)
+notation (xsymbols)
+  triples_valid  ("_|\<Turnstile>_:_" [61,0, 58] 57) and
+  ax_valid  ("_,_\<Turnstile>_" [61,58,58] 57)
 
 defs  triple_valid_def:  "G\<Turnstile>n:t  \<equiv> case t of {P} t\<succ> {Q} \<Rightarrow>
                           \<forall>Y s Z. P Y s Z \<longrightarrow> type_ok G t s \<longrightarrow>
                           (\<forall>Y' s'. G\<turnstile>s \<midarrow>t\<succ>\<midarrow>n\<rightarrow> (Y',s') \<longrightarrow> Q Y' s' Z)"
-translations         "G|\<Turnstile>n:ts" == "Ball ts (triple_valid G n)"
-defs   ax_valids_def:"G,A|\<Turnstile>ts  \<equiv>  \<forall>n. G|\<Turnstile>n:A \<longrightarrow> G|\<Turnstile>n:ts"
-translations         "G,A \<Turnstile>t"  == "G,A|\<Turnstile>{t}"
+
+defs  ax_valids_def:"G,A|\<Turnstile>ts  \<equiv>  \<forall>n. G|\<Turnstile>n:A \<longrightarrow> G|\<Turnstile>n:ts"
 
 lemma triple_valid_def2: "G\<Turnstile>n:{P} t\<succ> {Q} =  
  (\<forall>Y s Z. P Y s Z 
