src/HOL/Bali/Trans.thy
@@ -60,13 +60,13 @@ lemma the_var_AVar_simp:
 by (simp)
 declare the_var_AVar_def [simp del]
 
-syntax (xsymbols)
-  Ref  :: "loc \<Rightarrow> expr"
-  SKIP :: "expr"
+abbreviation
+  Ref :: "loc \<Rightarrow> expr"
+  where "Ref a == Lit (Addr a)"
 
-translations
-  "Ref a" == "Lit (Addr a)"
-  "SKIP"  == "Lit Unit"
+abbreviation
+  SKIP :: "expr"
+  where "SKIP == Lit Unit"
 
 inductive
   step :: "[prog,term \<times> state,term \<times> state] \<Rightarrow> bool" ("_\<turnstile>_ \<mapsto>1 _"[61,82,82] 81)
